proofs/talos/lean/Project/Beck/AnnotationMatches.lean
@@ -23,80 +23,80 @@ set_option maxHeartbeats 8000000
 
 namespace Project.Beck.AnnotationMatches
 
-def function_17_erase_copy_0_prefix_program : Wasm.Program :=
+def function_18_erase_copy_0_prefix_program : Wasm.Program :=
   Project.ProofKit.FixedArrayCopy.prefixProgram
     8 14
     11 15
 
-def function_17_erase_copy_0_suffix_program : Wasm.Program :=
+def function_18_erase_copy_0_suffix_program : Wasm.Program :=
   Project.ProofKit.FixedArrayCopy.suffixProgram
     1 8 14
     11 12
     15
 
-def function_17_erase_copy_0_program : Wasm.Program :=
+def function_18_erase_copy_0_program : Wasm.Program :=
   Project.ProofKit.FixedArrayCopy.program
     1 8 14
     11 12
     15
 
-theorem function_17_erase_copy_0_prefix_eq :
-    Project.ProofKit.Annotation.region Project.Beck.func17
+theorem function_18_erase_copy_0_prefix_eq :
+    Project.ProofKit.Annotation.region Project.Beck.func18
       [{ instructionIndex := 15, field := .thenBranch }] 53
-      56 = some function_17_erase_copy_0_prefix_program := by
+      56 = some function_18_erase_copy_0_prefix_program := by
   rfl
 
-theorem function_17_erase_copy_0_suffix_eq :
-    Project.ProofKit.Annotation.region Project.Beck.func17
+theorem function_18_erase_copy_0_suffix_eq :
+    Project.ProofKit.Annotation.region Project.Beck.func18
       [{ instructionIndex := 15, field := .thenBranch }] 56
-      59 = some function_17_erase_copy_0_suffix_program := by
+      59 = some function_18_erase_copy_0_suffix_program := by
   rfl
 
-theorem function_17_erase_copy_0_eq :
-    Project.ProofKit.Annotation.region Project.Beck.func17
+theorem function_18_erase_copy_0_eq :
+    Project.ProofKit.Annotation.region Project.Beck.func18
       [{ instructionIndex := 15, field := .thenBranch }] 53
-      59 = some function_17_erase_copy_0_program := by
+      59 = some function_18_erase_copy_0_program := by
   rfl
 
-theorem function_17_erase_copy_0_tail_eq :
-    ((Project.ProofKit.Annotation.resolve Project.Beck.func17 [{ instructionIndex := 15, field := .thenBranch }]).getD []).drop 53 =
-      Project.Beck.AnnotationMatches.function_17_erase_copy_0_program ++ ((Project.ProofKit.Annotation.resolve Project.Beck.func17 [{ instructionIndex := 15, field := .thenBranch }]).getD []).drop 59 := by
+theorem function_18_erase_copy_0_tail_eq :
+    ((Project.ProofKit.Annotation.resolve Project.Beck.func18 [{ instructionIndex := 15, field := .thenBranch }]).getD []).drop 53 =
+      Project.Beck.AnnotationMatches.function_18_erase_copy_0_program ++ ((Project.ProofKit.Annotation.resolve Project.Beck.func18 [{ instructionIndex := 15, field := .thenBranch }]).getD []).drop 59 := by
   rfl
 
-def function_18_while_loop_0_guard_program : Wasm.Program :=
+def function_19_while_loop_0_guard_program : Wasm.Program :=
   Project.ProofKit.FuelGuard.program 0 12
 
-theorem function_18_while_loop_0_guard_eq :
-    Project.ProofKit.Annotation.region Project.Beck.func18
-      [{ instructionIndex := 8, field := .block }, { instructionIndex := 0, field := .loop }] 0 7 = some function_18_while_loop_0_guard_program := by
+theorem function_19_while_loop_0_guard_eq :
+    Project.ProofKit.Annotation.region Project.Beck.func19
+      [{ instructionIndex := 8, field := .block }, { instructionIndex := 0, field := .loop }] 0 7 = some function_19_while_loop_0_guard_program := by
   rfl
 
-theorem function_18_while_loop_0_guard_tail_eq :
-    (Project.ProofKit.Annotation.resolve Project.Beck.func18 [{ instructionIndex := 8, field := .block }, { instructionIndex := 0, field := .loop }]).getD [] = function_18_while_loop_0_guard_program ++ ((Project.ProofKit.Annotation.resolve Project.Beck.func18 [{ instructionIndex := 8, field := .block }, { instructionIndex := 0, field := .loop }]).getD []).drop 7 := by
+theorem function_19_while_loop_0_guard_tail_eq :
+    (Project.ProofKit.Annotation.resolve Project.Beck.func19 [{ instructionIndex := 8, field := .block }, { instructionIndex := 0, field := .loop }]).getD [] = function_19_while_loop_0_guard_program ++ ((Project.ProofKit.Annotation.resolve Project.Beck.func19 [{ instructionIndex := 8, field := .block }, { instructionIndex := 0, field := .loop }]).getD []).drop 7 := by
   rfl
 
-def function_21_while_loop_0_guard_program : Wasm.Program :=
+def function_22_while_loop_0_guard_program : Wasm.Program :=
   Project.ProofKit.FuelGuard.program 0 17
 
-theorem function_21_while_loop_0_guard_eq :
-    Project.ProofKit.Annotation.region Project.Beck.func21
-      [{ instructionIndex := 8, field := .block }, { instructionIndex := 0, field := .loop }] 0 7 = some function_21_while_loop_0_guard_program := by
+theorem function_22_while_loop_0_guard_eq :
+    Project.ProofKit.Annotation.region Project.Beck.func22
+      [{ instructionIndex := 8, field := .block }, { instructionIndex := 0, field := .loop }] 0 7 = some function_22_while_loop_0_guard_program := by
   rfl
 
-theorem function_21_while_loop_0_guard_tail_eq :
-    (Project.ProofKit.Annotation.resolve Project.Beck.func21 [{ instructionIndex := 8, field := .block }, { instructionIndex := 0, field := .loop }]).getD [] = function_21_while_loop_0_guard_program ++ ((Project.ProofKit.Annotation.resolve Project.Beck.func21 [{ instructionIndex := 8, field := .block }, { instructionIndex := 0, field := .loop }]).getD []).drop 7 := by
+theorem function_22_while_loop_0_guard_tail_eq :
+    (Project.ProofKit.Annotation.resolve Project.Beck.func22 [{ instructionIndex := 8, field := .block }, { instructionIndex := 0, field := .loop }]).getD [] = function_22_while_loop_0_guard_program ++ ((Project.ProofKit.Annotation.resolve Project.Beck.func22 [{ instructionIndex := 8, field := .block }, { instructionIndex := 0, field := .loop }]).getD []).drop 7 := by
   rfl
 
-def function_26_while_loop_0_guard_program : Wasm.Program :=
+def function_28_while_loop_0_guard_program : Wasm.Program :=
   Project.ProofKit.FuelGuard.program 0 15
 
-theorem function_26_while_loop_0_guard_eq :
-    Project.ProofKit.Annotation.region Project.Beck.func26
-      [{ instructionIndex := 6, field := .block }, { instructionIndex := 0, field := .loop }] 0 7 = some function_26_while_loop_0_guard_program := by
+theorem function_28_while_loop_0_guard_eq :
+    Project.ProofKit.Annotation.region Project.Beck.func28
+      [{ instructionIndex := 6, field := .block }, { instructionIndex := 0, field := .loop }] 0 7 = some function_28_while_loop_0_guard_program := by
   rfl
 
-theorem function_26_while_loop_0_guard_tail_eq :
-    (Project.ProofKit.Annotation.resolve Project.Beck.func26 [{ instructionIndex := 6, field := .block }, { instructionIndex := 0, field := .loop }]).getD [] = function_26_while_loop_0_guard_program ++ ((Project.ProofKit.Annotation.resolve Project.Beck.func26 [{ instructionIndex := 6, field := .block }, { instructionIndex := 0, field := .loop }]).getD []).drop 7 := by
+theorem function_28_while_loop_0_guard_tail_eq :
+    (Project.ProofKit.Annotation.resolve Project.Beck.func28 [{ instructionIndex := 6, field := .block }, { instructionIndex := 0, field := .loop }]).getD [] = function_28_while_loop_0_guard_program ++ ((Project.ProofKit.Annotation.resolve Project.Beck.func28 [{ instructionIndex := 6, field := .block }, { instructionIndex := 0, field := .loop }]).getD []).drop 7 := by
   rfl
 
 end Project.Beck.AnnotationMatches
